examples/ProcDecInv.v
@@ -1,6 +1,6 @@
 Require Import Bool String List.
 Require Import Lib.CommonTactics Lib.ilist Lib.Word.
-Require Import Lib.Struct Lib.StringBound Lib.FMap Lib.StringEq Lib.Indexer.
+Require Import Lib.Struct Lib.StructNotation Lib.StringBound Lib.FMap Lib.StringEq Lib.Indexer.
 Require Import Kami.Syntax Kami.Semantics Kami.RefinementFacts Kami.Renaming Kami.Wf.
 Require Import Kami.Renaming Kami.Specialize Kami.Inline Kami.InlineFacts Kami.Decomposition.
 Require Import Kami.Tactics Kami.Notations.
@@ -10,11 +10,11 @@ Require Import Eqdep ProofIrrelevance.
 Set Implicit Arguments.
 
 Section Invariants.
-  Variables opIdx addrSize iaddrSize fifoSize lgDataBytes rfIdx: nat.
+  Variables opIdx addrSize fifoSize lgDataBytes rfIdx: nat.
 
-  Variable dec: DecT opIdx addrSize iaddrSize lgDataBytes rfIdx.
-  Variable execState: ExecStateT opIdx addrSize iaddrSize lgDataBytes rfIdx.
-  Variable execNextPc: ExecNextPcT opIdx addrSize iaddrSize lgDataBytes rfIdx.
+  Variable dec: DecT opIdx addrSize lgDataBytes rfIdx.
+  Variable execState: ExecStateT opIdx addrSize lgDataBytes rfIdx.
+  Variable execNextPc: ExecNextPcT opIdx addrSize lgDataBytes rfIdx.
 
   Variables opLd opSt opTh: ConstT (Bit opIdx).
   Hypothesis (HldSt: (if weq (evalConstT opLd) (evalConstT opSt) then true else false) = false).
@@ -24,11 +24,53 @@ Section Invariants.
 
   Definition pdecInl := pdecInl fifoSize dec execState execNextPc opLd opSt opTh.
 
-  Definition procDec_inv_0 (o: RegsT): Prop.
+  Definition fifo_empty_inv (fifoEmpty: bool) (fifoEnqP fifoDeqP: type (Bit fifoSize)): Prop :=
+    fifoEmpty = true /\ fifoEnqP = fifoDeqP.
+  
+  Definition fifo_not_empty_inv (fifoEmpty: bool) (fifoEnqP fifoDeqP: type (Bit fifoSize)): Prop :=
+    fifoEmpty = false /\ fifoEnqP = fifoDeqP ^+ $1.
+
+  Definition mem_request_inv
+             (instRaw: fullType type (SyntaxKind (Data lgDataBytes)))
+             (rf: fullType type (SyntaxKind (Vector (Data lgDataBytes) rfIdx)))
+             (insEmpty: bool) (insElt: type (Vector RqFromProc fifoSize))
+             (insDeqP: type (Bit fifoSize)): Prop.
   Proof.
-    kexistv "pc"%string pcv o (Bit iaddrSize).
+    refine (if insEmpty then True else _).
+    refine (_ /\ _ /\ _).
+    - refine (_ /\ _).
+      + exact ((if weq (evalExpr (dec _ rf instRaw) ``"opcode") (evalConstT opLd)
+                then false else true) = insElt insDeqP ``"op").
+      + exact ((if weq (evalExpr (dec _ rf instRaw) ``"opcode") (evalConstT opSt)
+                then true else false) = insElt insDeqP ``"op").
+    - exact (insElt insDeqP ``"addr" = evalExpr (dec _ rf instRaw) ``"addr").
+    - refine (if (insElt insDeqP ``"op") : bool then _ else _).
+      + exact (insElt insDeqP ``"data" = evalExpr (dec _ rf instRaw) ``"value").
+      + exact (insElt insDeqP ``"data" = evalConstT (getDefaultConst (Data lgDataBytes))).
+  Defined.
+
+  Definition fetch_request_inv
+             (pc: fullType type (SyntaxKind (Bit addrSize)))
+             (rf: fullType type (SyntaxKind (Vector (Data lgDataBytes) rfIdx)))
+             (insEmpty: bool) (insElt: type (Vector RqFromProc fifoSize))
+             (insDeqP: type (Bit fifoSize)): Prop.
+  Proof.
+    refine (if insEmpty then True else _).
+    refine (_ /\ _ /\ _).
+    - exact (insElt insDeqP ``"op" = false).
+    - exact (insElt insDeqP ``"addr" = pc).
+    - exact (insElt insDeqP ``"data" = evalConstT (getDefaultConst (Data lgDataBytes))).
+  Defined.
+  Hint Unfold fifo_empty_inv fifo_not_empty_inv mem_request_inv fetch_request_inv: InvDefs.
+
+  Definition procDec_inv (o: RegsT): Prop.
+  Proof.
+    kexistv "pc"%string pcv o (Bit addrSize).
     kexistv "rf"%string rfv o (Vector (Data lgDataBytes) rfIdx).
-    kexistv "stall"%string stallv o Bool.
+    kexistv "memStall"%string stallv o Bool.
+    kexistv "fetch"%string fetchv o Bool.
+    kexistv "fetched"%string fetchedv o (Data lgDataBytes).
+    kexistv "fetchStall"%string fstallv o Bool.
     kexistv "rqFromProc"--"empty"%string iev o Bool.
     kexistv "rqFromProc"--"full"%string ifv o Bool.
     kexistv "rqFromProc"--"enqP"%string ienqpv o (Bit fifoSize).
@@ -39,95 +81,43 @@ Section Invariants.
     kexistv "rsToProc"--"enqP"%string oenqpv o (Bit fifoSize).
     kexistv "rsToProc"--"deqP"%string odeqpv o (Bit fifoSize).
     kexistv "rsToProc"--"elt"%string oeltv o (Vector RsToProc fifoSize).
-    exact True.
+    refine (_ \/ _).
+    - (* fetch stage *)
+      refine (fetchv = true /\ stallv = false /\ (or3 _ _ _)).
+      + (* reqInstFetch *)
+        exact (fstallv = false /\
+               fifo_empty_inv iev ienqpv ideqpv /\
+               fifo_empty_inv oev oenqpv odeqpv).
+      + (* processLd *)
+        refine (_ /\ _).
+        * exact (fstallv = true /\
+                 fifo_not_empty_inv iev ienqpv ideqpv /\
+                 fifo_empty_inv oev oenqpv odeqpv).
+        * exact (fetch_request_inv pcv rfv iev ieltv ideqpv).
+      + (* repInstFetch *)
+        exact (fstallv = true /\
+               fifo_empty_inv iev ienqpv ideqpv /\
+               fifo_not_empty_inv oev oenqpv odeqpv).
+    - (* execute stage *)
+      refine (fetchv = false /\ fstallv = false /\ (or3 _ _ _)).
+      + (* reqLd/St *)
+        exact (stallv = false /\
+               fifo_empty_inv iev ienqpv ideqpv /\
+               fifo_empty_inv oev oenqpv odeqpv).
+      + (* processLd/St *)
+        refine (_ /\ _).
+        * exact (stallv = true /\
+                 fifo_not_empty_inv iev ienqpv ideqpv /\
+                 fifo_empty_inv oev oenqpv odeqpv).
+        * exact (mem_request_inv fetchedv rfv iev ieltv ideqpv).
+      + (* repLd/St *)
+        exact (stallv = true /\
+               fifo_empty_inv iev ienqpv ideqpv /\
+               fifo_not_empty_inv oev oenqpv odeqpv).
   Defined.
-  Hint Unfold procDec_inv_0: InvDefs.
+  Hint Unfold procDec_inv: InvDefs.
 
-  Definition fifo_empty_inv (fifoEmpty: bool) (fifoEnqP fifoDeqP: type (Bit fifoSize)): Prop :=
-    fifoEmpty = true /\ fifoEnqP = fifoDeqP.
-  
-  Definition fifo_not_empty_inv (fifoEmpty: bool) (fifoEnqP fifoDeqP: type (Bit fifoSize)): Prop :=
-    fifoEmpty = false /\ fifoEnqP = fifoDeqP ^+ $1.
-
-  Definition mem_request_inv
-             (pc: fullType type (SyntaxKind (Bit iaddrSize)))
-             (rf: fullType type (SyntaxKind (Vector (Data lgDataBytes) rfIdx)))
-             (insEmpty: bool) (insElt: type (Vector RqFromProc fifoSize))
-             (insDeqP: type (Bit fifoSize)): Prop.
-  Proof.
-    refine (if insEmpty then True else _).
-    refine (_ /\ _ /\ _).
-    - refine (_ /\ _).
-      + exact ((if weq (evalExpr (dec _ rf pc) {| bindex := "opcode"%string |}) (evalConstT opLd)
-                then false else true) = insElt insDeqP {| bindex := "op"%string |}).
-      + exact ((if weq (evalExpr (dec _ rf pc) {| bindex := "opcode"%string |}) (evalConstT opSt)
-                then true else false) = insElt insDeqP {| bindex := "op"%string |}).
-    - exact (insElt insDeqP {| bindex := "addr"%string |} =
-             evalExpr (dec _ rf pc) {| bindex := "addr"%string |}).
-    - refine (if (insElt insDeqP {| bindex := "op"%string |}) : bool then _ else _).
-      + exact (insElt insDeqP {| bindex := "data"%string |} =
-               evalExpr (dec _ rf pc)
-                        {| bindex := "value"%string |}).
-      + exact (insElt insDeqP {| bindex := "data"%string |} =
-               evalConstT (getDefaultConst (Data lgDataBytes))).
-  Defined.
-  Hint Unfold fifo_empty_inv fifo_not_empty_inv mem_request_inv: InvDefs.
-
-  Definition procDec_inv_1 (o: RegsT): Prop.
-  Proof.
-    kexistv "pc"%string pcv o (Bit iaddrSize).
-    kexistv "rf"%string rfv o (Vector (Data lgDataBytes) rfIdx).
-    kexistv "stall"%string stallv o Bool.
-    kexistv "rqFromProc"--"empty"%string iev o Bool.
-    kexistv "rqFromProc"--"enqP"%string ienqP o (Bit fifoSize).
-    kexistv "rqFromProc"--"deqP"%string ideqP o (Bit fifoSize).
-    kexistv "rqFromProc"--"elt"%string ieltv o (Vector RqFromProc fifoSize).
-    kexistv "rsToProc"--"empty"%string oev o Bool.
-    kexistv "rsToProc"--"enqP"%string oenqP o (Bit fifoSize).
-    kexistv "rsToProc"--"deqP"%string odeqP o (Bit fifoSize).
-    refine (or3 _ _ _).
-    - exact (v1 = false /\ fifo_empty_inv v2 v3 v4 /\ fifo_empty_inv v6 v7 v8).
-    - refine (_ /\ _).
-      + exact (v1 = true /\ fifo_not_empty_inv v2 v3 v4 /\ fifo_empty_inv v6 v7 v8).
-      + exact (mem_request_inv v v0 v2 v5 v4).
-    - exact (v1 = true /\ fifo_empty_inv v2 v3 v4 /\ fifo_not_empty_inv v6 v7 v8).
-  Defined.
-  Hint Unfold procDec_inv_1: InvDefs.
-
-  Lemma procDec_inv_0_ok':
-    forall init n ll,
-      init = initRegs (getRegInits (fst pdecInl)) ->
-      Multistep (fst pdecInl) init n ll ->
-      procDec_inv_0 n.
-  Proof. (* SKIP_PROOF_ON
-    induction 2.
-
-    - kinv_magic_light.
-
-    - kinvert.
-      + kinv_magic_light.
-      + kinv_magic_light.
-      + kinv_magic_light.
-      + kinv_magic_light.
-      + kinv_magic_light.
-      + kinv_magic_light.
-      + kinv_magic_light.
-      + kinv_magic_light.
-      + kinv_magic_light.
-      + kinv_magic_light.
-        END_SKIP_PROOF_ON *) admit.
-  Qed.
-
-  Lemma procDec_inv_0_ok:
-    forall o,
-      reachable o (fst pdecInl) ->
-      procDec_inv_0 o.
-  Proof.
-    intros; inv H; inv H0.
-    eapply procDec_inv_0_ok'; eauto.
-  Qed.
-
-  Ltac procDec_inv_1_tac :=
+  Ltac procDec_inv_tac :=
     kinv_or3;
     repeat
       match goal with
@@ -135,55 +125,75 @@ Section Invariants.
       | [ |- exists _, _ ] => eexists
       end.
 
-  Lemma procDec_inv_1_ok':
+  Lemma procDec_inv_ok':
     forall init n ll,
       init = initRegs (getRegInits (fst pdecInl)) ->
       Multistep (fst pdecInl) init n ll ->
-      procDec_inv_1 n.
+      procDec_inv n.
   Proof. (* SKIP_PROOF_ON
     induction 2.
 
-    - kinv_magic_light_with procDec_inv_1_tac.
-      or3_fst; kinv_magic_light_with procDec_inv_1_tac.
+    - kinv_magic_light_with procDec_inv_tac.
+      left; repeat split; auto; or3_fst.
+      kinv_magic_light_with procDec_inv_tac.
 
     - kinvert.
       + mred.
       + mred.
       + kinv_magic_light_with kinv_or3.
-        or3_snd; kinv_magic_light_with procDec_inv_1_tac.
+        left; repeat split; auto; or3_snd.
+        kinv_magic_light_with procDec_inv_tac.
+      + kinv_magic_light_with kinv_or3.
+        right; repeat split; auto; or3_fst.
+        kinv_magic_light_with procDec_inv_tac.
+      + kinv_magic_light_with kinv_or3.
+        right; repeat split; auto; or3_snd.
+        kinv_magic_light_with procDec_inv_tac.
         * kinv_finish.
         * kinv_finish.
       + kinv_magic_light_with kinv_or3.
-        or3_snd; kinv_magic_light_with procDec_inv_1_tac.
+        right; repeat split; auto; or3_snd.
+        kinv_magic_light_with procDec_inv_tac.
         * kinv_finish.
         * kinv_finish.
       + kinv_magic_light_with kinv_or3.
-        or3_fst; kinv_magic_light_with procDec_inv_1_tac.
+        left; repeat split; auto; or3_fst.
+        kinv_magic_light_with procDec_inv_tac.
       + kinv_magic_light_with kinv_or3.
-        or3_fst; kinv_magic_light_with procDec_inv_1_tac.
+        left; repeat split; auto; or3_fst.
+        kinv_magic_light_with procDec_inv_tac.
       + kinv_magic_light_with kinv_or3.
-        or3_fst; kinv_magic_light_with procDec_inv_1_tac.
+        left; repeat split; auto; or3_fst.
+        kinv_magic_light_with procDec_inv_tac.
       + kinv_magic_light_with kinv_or3.
-        or3_fst; kinv_magic_light_with procDec_inv_1_tac.
+        left; repeat split; auto; or3_fst.
+        kinv_magic_light_with procDec_inv_tac.
       + kinv_magic_light_with kinv_or3.
-        or3_thd; kinv_magic_light_with procDec_inv_1_tac.
+        * left; repeat split; auto; or3_thd.
+          kinv_magic_light_with procDec_inv_tac.
+        * right; repeat split; auto; or3_thd.
+          kinv_magic_light_with procDec_inv_tac.
       + kinv_magic_light_with kinv_or3.
-        or3_thd; kinv_magic_light_with procDec_inv_1_tac.
-        END_SKIP_PROOF_ON *) admit.
+        * left; repeat split; auto; or3_thd.
+          kinv_magic_light_with procDec_inv_tac.
+        * right; repeat split; auto; or3_thd.
+          kinv_magic_light_with procDec_inv_tac.
+
+          END_SKIP_PROOF_ON *) admit.
   Qed.
 
-  Lemma procDec_inv_1_ok:
+  Lemma procDec_inv_ok:
     forall o,
       reachable o (fst pdecInl) ->
-      procDec_inv_1 o.
+      procDec_inv o.
   Proof.
     intros; inv H; inv H0.
-    eapply procDec_inv_1_ok'; eauto.
+    eapply procDec_inv_ok'; eauto.
   Qed.
 
 End Invariants.
 
 Hint Unfold RqFromProc RsToProc: MethDefs.
-Hint Unfold procDec_inv_0 procDec_inv_1
-     fifo_empty_inv fifo_not_empty_inv mem_request_inv: InvDefs.
+Hint Unfold procDec_inv fifo_empty_inv fifo_not_empty_inv
+     mem_request_inv fetch_request_inv: InvDefs.
 
