examples/ProcDecSC.v
@@ -1,6 +1,6 @@
 Require Import Bool String List.
 Require Import Lib.CommonTactics Lib.ilist Lib.Word.
-Require Import Lib.Struct Lib.StringBound Lib.FMap Lib.StringEq Lib.Indexer.
+Require Import Lib.Struct Lib.StructNotation Lib.StringBound Lib.FMap Lib.StringEq Lib.Indexer.
 Require Import Kami.Syntax Kami.Semantics Kami.RefinementFacts Kami.Renaming Kami.Wf.
 Require Import Kami.Renaming Kami.Inline Kami.InlineFacts.
 Require Import Kami.Decomposition Kami.Notations Kami.Tactics.
@@ -11,11 +11,11 @@ Require Import Eqdep.
 Set Implicit Arguments.
 
 Section ProcDecSC.
-  Variables opIdx addrSize iaddrSize fifoSize lgDataBytes rfIdx: nat.
+  Variables opIdx addrSize fifoSize lgDataBytes rfIdx: nat.
 
-  Variable dec: DecT opIdx addrSize iaddrSize lgDataBytes rfIdx.
-  Variable execState: ExecStateT opIdx addrSize iaddrSize lgDataBytes rfIdx.
-  Variable execNextPc: ExecNextPcT opIdx addrSize iaddrSize lgDataBytes rfIdx.
+  Variable dec: DecT opIdx addrSize lgDataBytes rfIdx.
+  Variable execState: ExecStateT opIdx addrSize lgDataBytes rfIdx.
+  Variable execNextPc: ExecNextPcT opIdx addrSize lgDataBytes rfIdx.
 
   Variables opLd opSt opTh: ConstT (Bit opIdx).
   Hypotheses (HldSt: (if weq (evalConstT opLd) (evalConstT opSt) then true else false) = false).
@@ -29,53 +29,99 @@ Section ProcDecSC.
   Hint Extern 1 (ModEquiv type typeUT pdec) => unfold pdec. (* for kequiv *)
   Hint Extern 1 (ModEquiv type typeUT pinst) => unfold pinst. (* for kequiv *)
 
-  Definition pdec_pinst_ruleMap (_: RegsT): string -> option string :=
-    "execToHost" |-> "execToHost";
-    "execNm"     |-> "execNm";
-    "processLd"  |-> "execLd";
-    "processSt"  |-> "execSt"; ||.
+  Definition pdec_pinst_ruleMap (o: RegsT): string -> option string.
+    refine ("execToHost" |-> "execToHost";
+            "execNm"     |-> "execNm";
+            "processSt"  |-> "execSt"; _).
+    kgetv "fetch"%string fetchv o Bool (fun _ : string => @None string).
+    exact (if fetchv
+           then "processLd" |-> "instFetch"; ||
+           else "processLd" |-> "execLd"; ||).
+  Defined.
+  Hint Unfold pdec_pinst_ruleMap: MethDefs.
 
   Definition pdec_pinst_regMap (r: RegsT): RegsT.
   Proof.
-    kgetv "pc"%string pcv r (Bit iaddrSize) (M.empty (sigT (fullType type))).
+    kgetv "pc"%string pcv r (Bit addrSize) (M.empty (sigT (fullType type))).
     kgetv "rf"%string rfv r (Vector (Data lgDataBytes) rfIdx) (M.empty (sigT (fullType type))).
+    kgetv "fetch"%string fetchv r Bool (M.empty (sigT (fullType type))).
+    kgetv "fetched"%string fetchedv r (Data lgDataBytes) (M.empty (sigT (fullType type))).
     kgetv "rsToProc"--"empty"%string oev r Bool (M.empty (sigT (fullType type))).
     kgetv "rsToProc"--"elt"%string oelv r (Vector RsToProc fifoSize)
           (M.empty (sigT (fullType type))).
     kgetv "rsToProc"--"deqP"%string odv r (Bit fifoSize) (M.empty (sigT (fullType type))).
 
-    pose proof (evalExpr (dec _ rfv pcv)) as inst.
-    refine (
-        if oev
-        then (M.add "pc"%string (existT _ _ pcv)
-                    (M.add "rf"%string (existT _ _ rfv)
-                           (M.empty _)))
-        else (M.add "pc"%string (existT _ _ (evalExpr (execNextPc _ rfv pcv inst)))
-                    (M.add "rf"%string _ (M.empty _)))
-      ).
+    refine (if oev
+            then (M.add "pc"%string (existT _ _ pcv)
+                        (M.add "rf"%string (existT _ _ rfv)
+                               (M.add "fetch"%string (existT _ _ fetchv)
+                                      (M.add "fetched"%string (existT _ _ fetchedv)
+                                             (M.empty _)))))
+            else _).
+    refine (if fetchv then _ else _).
 
-    pose proof (inst {| bindex := "opcode"%string |}) as opc.
-    destruct (weq opc (evalConstT opLd)).
-    - refine (existT _ (SyntaxKind (Vector (Data lgDataBytes) rfIdx)) _); simpl.
-      exact (fun a => if weq a (inst {| bindex := "reg"%string |})
-                      then (oelv odv) {| bindex := "data"%string |}
-                      else rfv a).
-    - refine (existT _ _ rfv).
+    - refine (M.add "pc"%string (existT _ _ pcv)
+                    (M.add "rf"%string (existT _ _ rfv)
+                           (M.add "fetch"%string (existT _ (SyntaxKind Bool) false)
+                                  (M.add "fetched"%string
+                                         (existT _ (SyntaxKind (Data lgDataBytes))
+                                                 (oelv odv ``"data"))
+                                         (M.empty _))))).
+
+    - pose proof (evalExpr (dec _ rfv fetchedv)) as inst.
+      refine (M.add "pc"%string (existT _ _ (evalExpr (execNextPc _ rfv pcv inst)))
+                    (M.add "rf"%string _
+                           (M.add "fetch"%string (existT _ (SyntaxKind Bool) true)
+                                  (M.add "fetched"%string (existT _ _ fetchedv)
+                                         (M.empty _))))).
+      pose proof (inst ``"opcode") as opc.
+      destruct (weq opc (evalConstT opLd)).
+      + refine (existT _ (SyntaxKind (Vector (Data lgDataBytes) rfIdx)) _); simpl.
+        exact (fun a => if weq a (inst ``"reg")
+                        then oelv odv ``"data"
+                        else rfv a).
+      + refine (existT _ _ rfv).
   Defined.
   Hint Unfold pdec_pinst_regMap: MethDefs. (* for kdecompose_regMap_init *)
 
-  Definition decInstConfig :=
-    {| inlining := true;
-       decomposition :=
-         DTFunctional pdec_pinst_regMap pdec_pinst_ruleMap;
-       invariants :=
-         IVCons procDec_inv_0_ok (IVCons procDec_inv_1_ok IVNil)
-    |}.
+  (* Definition decInstConfig := *)
+  (*   {| inlining := true; *)
+  (*      decomposition := DTFunctional pdec_pinst_regMap pdec_pinst_ruleMap; *)
+  (*      invariants := IVCons procDec_inv_ok IVNil *)
+  (*   |}. *)
 
   Lemma pdec_refines_pinst: pdec <<== pinst.
   Proof. (* SKIP_PROOF_ON
-    kami_ok decInstConfig kinv_or3.
-    END_SKIP_PROOF_ON *) admit.
+
+    kinline_left im.
+    kdecompose_nodefs pdec_pinst_regMap pdec_pinst_ruleMap.
+
+    kinv_add procDec_inv_ok.
+    kinv_add_end.
+
+    kinvert.
+    - kinv_magic_with kinv_or3.
+    - kinv_magic_with kinv_or3.
+    - kinv_magic_with kinv_or3.
+    - kinv_magic_with kinv_or3.
+    - kinv_magic_with kinv_or3.
+    - kinv_magic_with kinv_or3.
+    - kinv_magic_with kinv_or3.
+    - kinv_magic_with kinv_or3.
+    - kinv_magic_with kinv_or3.
+    - kinv_action_dest;
+        kinv_custom kinv_or3;
+        kinv_regmap_red.
+      + (* TODO: automation *)
+        unfold IndexBound_head, IndexBound_tail, mapAttr, addFirstBoundedIndex, bindex in *.
+        simpl in *.
+        rewrite H17 in H25.
+        kinv_contra.
+      + kinv_constr;
+          kinv_eq;
+          kinv_finish.
+
+        END_SKIP_PROOF_ON *) admit.
   Qed.
 
 End ProcDecSC.
